More MFES stuff

MFES/MFESTP5.dfy
@@ -5,36 +5,70 @@ class {:autocontracts} Deque {
     const list: array<T>; // circular array, from list[start] (front) to list[(start+size-1) % list.Length] (back) 
     var start : nat; 
     var size : nat;
+    ghost var elems: seq<T>;
+    ghost const capacity: nat;
+
+    predicate Valid(){
+        0 <= size <= list.Length
+      && 0<=start<list.Length
+      && (elems == if start+size <= list.Length then list[start..start+size] else list[start..] + list[..size-(list.Length-start)])
+      && capacity == list.Length 
+    }
  
-    constructor (capacity: nat) {
+    constructor (capacity: nat) 
+        requires capacity > 0
+        ensures Valid() && this.elems == [] && this.capacity == capacity
+    {
         list := new T[capacity];
         start := 0;
         size := 0;
+        this.elems := [];
+        this.capacity := capacity;
     }
  
-    predicate method isEmpty() {
+    predicate method isEmpty() 
+        requires Valid();
+        ensures this.elems == [];
+    {
         size == 0
     }
     
-    predicate method isFull() {
+    predicate method isFull() 
+        requires Valid();
+        ensures Valid() && |this.elems| == this.capacity    
+    {
         size == list.Length
     }
  
-    function method front() : T {
+    function method front() : T 
+        requires !isEmpty();
+        ensures front() == this.elems[0]; 
+    {
         list[start]
     }
  
-    function method back() : T {
+    function method back() : T 
+        requires !isEmpty();
+        ensures back() == this.elems[|this.elems| - 1]
+    {
         list[(start + size - 1) % list.Length] 
     }
     
-    method push_back(x : T) {
+    method push_back(x : T) 
+        requires !isFull();
+        ensures back() == x && this.elems == old(elems) + [x];
+    {
         list[(start + size) % list.Length] := x;
         size := size + 1;
+        elems := elems + [x];
     }
  
-    method pop_back() {
+    method pop_back() 
+        requires !isEmpty();
+        ensures elems == old(elems[..|elems|-1]);
+    {
         size := size - 1;
+        elems := elems[..|elems|-1];
     }
  
     method push_front(x : T) {
