MFES/FCULEXERCISE1.dfy
@@ -1,0 +1,21 @@
+method odd ( n: nat ) returns (j:int)
+    ensures j == 1 + 2 ∗ n
+    ensures j > n
+    ensures j % 2 == 1 // significa que j e impar, e a de cima ja garante isso
+{
+    var k := 0;
+    j := 1;
+
+    // I ^ not(C) => Q
+
+    // I ^ k >= n => j == 1 + 2 * n
+
+    while k < n
+        invariant k <= n;
+        invariant j == 1+2*k;
+        decreases n-k;
+    {
+        k := k + 1;
+        j := j + 2;
+    }
+}
