MFES/FCULEXERCISE2.dfy
@@ -1,0 +1,18 @@
+method squareRoot ( n: nat ) returns ( r: nat )
+    ensures r ∗ r <= n < (r+1) ∗ (r+1)
+{
+    r := 0;
+    var sqr := 1;
+
+    //  I ^ (sqr > n) => r ∗ r <= n < ( r + 1 ) ∗ ( r + 1 )
+
+    while sqr <= n
+        invariant r < sqr;
+        invariant r*r <= n;
+        invariant sqr == (r+1) * (r+1);
+        decreases n-sqr;
+    {
+        r := r + 1;
+        sqr := sqr + 2 ∗ r + 1;
+    }
+}
