MFES/FCULEXERCISE3.dfy
@@ -1,0 +1,21 @@
+function powerOfTwo (n: nat) : nat
+    decreases n;
+{
+    if n == 0 then 1 else 2*powerOfTwo(n-1) 
+}
+
+method power ( n: nat ) returns ( j : nat )
+    ensures j == powerOfTwo(n);
+{
+    var k := 0;
+    j := 1;
+
+    while k < n
+        invariant k <= n;
+        invariant j == powerOfTwo(k);
+        decreases n-k;
+    {
+        k := k + 1;
+        j := 2 ∗ j ;
+    }
+}
