MFES/FCULEXERCISES5.dfy
@@ -1,0 +1,17 @@
+method divide ( x : nat , y : nat ) returns ( q : nat , r : nat )
+    requires y > 0;
+    ensures q ∗ y + r == x && r >= 0 && r < y ;
+{
+    q := 0;
+    r := x ;
+
+    // I ^ r < y ==> q ∗ y + r == x && r >= 0 && r < y 
+
+    while r >= y 
+        invariant q ∗ y + r == x && r >= 0; 
+        decreases r;
+    {
+        r := r − y ;
+        q := q + 1;
+    }
+}
