MFES/FCULEXERCISES6.dfy
@@ -1,0 +1,10 @@
+method p rodu ct (m: nat , n: i n t ) re turns ( p: i n t )
+ensures p == m ∗ n ;
+{
+var i : nat := m;
+p := 0;
+while ( i != 0 ) {
+p := p + n ;
+i := i − 1;
+}
+}
